src/Init/Data/Iterators/Lemmas/Combinators/Monadic/Scan.lean
@@ -19,31 +19,31 @@ public section
 namespace Std
 open Std.Internal Std.Iterators Std.Iterators.Types
 
-theorem IterM.InternalCombinators.step_scanM
+theorem IterM.Intermediate.step_scanM
     {f : γ → β → PostconditionT n γ} [Iterator α m β] [MonadLiftT m n] [Monad n]
     {it : IterM (α := α) m β} {acc : γ} {yieldAcc : Bool} :
-    (IterM.InternalCombinators.scanM f acc yieldAcc it).step = (do
+    (IterM.Intermediate.scanM f acc yieldAcc it).step = (do
         if h : yieldAcc = true then
           return .deflate <| .yield
-            (IterM.InternalCombinators.scanM f acc false it)
+            (IterM.Intermediate.scanM f acc false it)
             acc
-            (.yieldAcc (by simp [IterM.InternalCombinators.scanM, h]))
+            (.yieldAcc (by simp [IterM.Intermediate.scanM, h]))
         else
           match (← it.step).inflate with
           | .yield it' b hp => do
             let ⟨newAcc, h_acc⟩ ← (f acc b).operation
             return .deflate <| .yield
-              (IterM.InternalCombinators.scanM f newAcc false it')
+              (IterM.Intermediate.scanM f newAcc false it')
               newAcc
-              (.yieldNext (by simp [IterM.InternalCombinators.scanM, h]) hp h_acc)
+              (.yieldNext (by simp [IterM.Intermediate.scanM, h]) hp h_acc)
           | .skip it' hp =>
             return .deflate <| .skip
-              (IterM.InternalCombinators.scanM f acc false it')
-              (.skip (by simp [IterM.InternalCombinators.scanM, h]) hp)
+              (IterM.Intermediate.scanM f acc false it')
+              (.skip (by simp [IterM.Intermediate.scanM, h]) hp)
           | .done hp =>
             return .deflate <|
-              .done (.done (by simp [IterM.InternalCombinators.scanM, h]) hp)) := by
-  simp only [IterM.InternalCombinators.scanM, IterM.step_eq]
+              .done (.done (by simp [IterM.Intermediate.scanM, h]) hp)) := by
+  simp only [IterM.Intermediate.scanM, IterM.step_eq]
   cases h : yieldAcc
   case true => rfl
   case false =>
@@ -54,17 +54,17 @@ theorem IterM.InternalCombinators.step_scanM
 private theorem IterM.toList_scanWithPostCondition_afterInit
     [Monad m] [LawfulMonad m] [Iterator α Id β] [Finite α Id]
     {f : γ → β → PostconditionT m γ} {init : γ} (it : IterM (α := α) Id β) :
-    IterM.toList (IterM.InternalCombinators.scanM (m := Id) f init false it) =
+    IterM.toList (IterM.Intermediate.scanM (m := Id) f init false it) =
       return ((← it.toList.run.scanlM (f · · |>.run) init).tail) := by
   induction it using IterM.inductSteps generalizing init with | step it ihy ihs =>
   rw [IterM.toList_eq_match_step, IterM.toList_eq_match_step]
-  simp only [IterM.InternalCombinators.step_scanM, ↓reduceDIte, Bool.false_eq_true]
+  simp only [IterM.Intermediate.step_scanM, ↓reduceDIte, Bool.false_eq_true]
   simp only [monadLift, liftM, PostconditionT.run_eq_map] at *
   match hstep : it.step.run.inflate with
   | ⟨.yield inner' out, hp⟩ =>
     simp only [bind_pure_comp, pure_bind, hstep, bind_map_left, Shrink.inflate_deflate, Id.run_bind,
       Id.run_map, List.scanlM_cons, map_bind, ihy hp]
-    simp +singlePass only [← List.scanlM_cons_head_tail]
+    simp +singlePass only [← List.cons_tail_scanlM]
     simp
   | ⟨.skip inner, hp⟩ => simp_all
   | ⟨.done, x⟩ => simp_all
@@ -72,11 +72,11 @@ private theorem IterM.toList_scanWithPostCondition_afterInit
 private theorem IterM.toList_scan_afterInit
     [Monad m] [LawfulMonad m] [Iterator α m β] [Finite α m]
     {f : γ → β → γ} {init : γ} (it : IterM (α := α) m β) :
-    IterM.toList (IterM.InternalCombinators.scanM (pure <| f · ·) init false it) =
+    IterM.toList (IterM.Intermediate.scanM (pure <| f · ·) init false it) =
       (List.scanl f init · |>.tail) <$> it.toList := by
   induction it using IterM.inductSteps generalizing init with | step it ihy ihs =>
   rw [IterM.toList_eq_match_step, IterM.toList_eq_match_step]
-  simp only [IterM.InternalCombinators.step_scanM, ↓reduceDIte, Bool.false_eq_true]
+  simp only [IterM.Intermediate.step_scanM, ↓reduceDIte, Bool.false_eq_true]
   simp only [monadLift, liftM] at *
   simp only [bind_assoc, map_eq_pure_bind]
   apply bind_congr; intro step
@@ -84,7 +84,7 @@ private theorem IterM.toList_scan_afterInit
   | ⟨.yield inner' out, hp⟩ =>
     simp only [PostconditionT.operation_pure, bind_pure_comp, map_pure,
       pure_bind, Shrink.inflate_deflate, ihy hp, Functor.map_map, List.scanl_cons, List.tail_cons]
-    simp +singlePass only [← List.scanl_cons_head_tail]
+    simp +singlePass only [← List.cons_tail_scanl]
     simp
   | ⟨.skip inner, hp⟩ => simp_all
   | ⟨.done, x⟩ => simp_all
@@ -94,9 +94,9 @@ theorem IterM.toList_scanWithPostCondition [Monad m] [LawfulMonad m] [Iterator �
     {f : γ → β → PostconditionT m γ} {init : γ} (it : IterM (α := α) Id β) :
     (it.scanWithPostcondition f init).toList = it.toList.run.scanlM (f · · |>.run) init := by
   unfold IterM.scanWithPostcondition
-  rw [IterM.toList_eq_match_step, IterM.InternalCombinators.step_scanM]
+  rw [IterM.toList_eq_match_step, IterM.Intermediate.step_scanM]
   simp only [↓reduceDIte, pure_bind, Shrink.inflate_deflate]
-  rw [toList_scanWithPostCondition_afterInit, ← List.scanlM_cons_head_tail]
+  rw [toList_scanWithPostCondition_afterInit, ← List.cons_tail_scanlM]
   simp
 
 @[simp]
@@ -110,11 +110,11 @@ theorem IterM.toList_scan [Iterator α m β] [Finite α m] [Monad m] [LawfulMona
     {f : γ → β → γ} {init : γ} (it : IterM (α := α) m β) :
     (it.scan f init).toList = List.scanl f init <$> it.toList := by
   rw [scan, scanWithPostcondition]
-  rw [IterM.toList_eq_match_step, IterM.InternalCombinators.step_scanM]
+  rw [IterM.toList_eq_match_step, IterM.Intermediate.step_scanM]
   simp only [↓reduceDIte, pure_bind, Shrink.inflate_deflate,
     toList_scan_afterInit, bind_pure_comp, Functor.map_map]
   congr 1; apply funext
-  simp +singlePass only [← List.scanl_cons_head_tail]
+  simp +singlePass only [← List.cons_tail_scanl]
   simp
 
 end Std
