src/Init/Data/Iterators/Lemmas/Combinators/Scan.lean
@@ -14,10 +14,39 @@ import Init.Data.Iterators.Lemmas.Combinators.Monadic.Scan
 public section
 
 namespace Std
-open Std.Iterators
+open Std.Iterators Std.Iterators.Types
 
 variable {α β γ : Type w} [Iterator α Id β] {it : Iter (α := α) β}
-    {m : Type w → Type w'}
+
+theorem Iter.Intermediate.step_scanM [Monad m] [LawfulMonad m]
+    {f : γ → β → PostconditionT m γ} {acc : γ} {yieldAcc : Bool} :
+    (IterM.Intermediate.scanM f acc yieldAcc it.toIterM).step = (do
+        if h : yieldAcc = true then
+          return .deflate <| .yield
+            (IterM.Intermediate.scanM f acc false it.toIterM)
+            acc
+            (.yieldAcc (by simp [IterM.Intermediate.scanM, h]))
+        else
+          match it.step with
+          | .yield it' b hp => do
+            let ⟨newAcc, h_acc⟩ ← (f acc b).operation
+            return .deflate <| .yield
+              (IterM.Intermediate.scanM f newAcc false it'.toIterM)
+              newAcc
+              (.yieldNext (by simp [IterM.Intermediate.scanM, h]) hp h_acc)
+          | .skip it' hp =>
+            return .deflate <| .skip
+              (IterM.Intermediate.scanM f acc false it'.toIterM)
+              (.skip (by simp [IterM.Intermediate.scanM, h]) hp)
+          | .done hp =>
+            return .deflate <|
+              .done (.done (by simp [IterM.Intermediate.scanM, h]) hp)) := by
+  simp only [IterM.Intermediate.step_scanM]
+  cases h : yieldAcc
+  case true => rfl
+  case false =>
+    simp only [monadLift, liftM, pure_bind, Iter.step]
+    cases it.toIterM.step.run.inflate using PlausibleIterStep.casesOn <;> simp
 
 @[simp]
 theorem Iter.toList_scanWithPostcondition [Monad m] [LawfulMonad m] [Finite α Id]
