src/Init/Data/List/Scan/Lemmas.lean
@@ -51,7 +51,7 @@ theorem scanlM_cons [Monad m] [LawfulMonad m] {f : α → β → m α} :
     scanlM f init (x :: xs) = return init :: (← scanlM f (← f init x) xs) := by
   simp [scanlM, scanAuxM_cons]
 
-theorem scanlM_cons_head_tail [Monad m] [LawfulMonad m]
+theorem cons_tail_scanlM [Monad m] [LawfulMonad m]
     {f : γ → β → m γ} {init : γ} {as : List β} :
     (return (init :: (← as.scanlM f init).tail)) = as.scanlM f init := by
   induction as generalizing init with simp_all
@@ -133,8 +133,7 @@ theorem scanl_nil {f : β → α → β} : scanl f init [] = [init] := by simp [
 theorem scanl_cons {f : β → α → β} : scanl f b (a :: l) = b :: scanl f (f b a) l := by
   simp [scanl]
 
-theorem scanl_cons_head_tail
-    {f : γ → β → γ} {init : γ} {as : List β} :
+theorem cons_tail_scanl {f : γ → β → γ} {init : γ} {as : List β} :
     init :: (as.scanl f init).tail = as.scanl f init := by
   induction as generalizing init with simp_all
 
